@prefix dct: <http://purl.org/dc/terms/> .
@prefix me: <http://example.org/taxonomy/> .
@prefix skos: <http://www.w3.org/2004/02/skos/core#> .
@prefix vann: <http://purl.org/vocab/vann/> .

me:mechanical a skos:Concept ;
    skos:broader me:Property ;
    skos:definition "Properties of materials that are related to their mechanical behavior, such as strength, elasticity, and durability."@en ;
    skos:inScheme me:MyThesaurus ;
    skos:prefLabel "Mechanisch"@de,
        "Mechanical"@en,
        "Mécanique"@fr .

me:density a skos:Concept ;
    skos:broader me:mechanical ;
    skos:definition "Density of a material, defined as its mass per unit volume."@en ;
    skos:inScheme me:MyThesaurus ;
    skos:prefLabel "Dichte"@de,
        "Density"@en,
        "Densité"@fr .

me:compressiveStrength a skos:Concept ;
    skos:broader me:mechanical ;
    skos:definition "The ability of a material to withstand axial loads without failure."@en ;
    skos:inScheme me:MyThesaurus ;
    skos:prefLabel "Druckfestigkeit"@de,
        "Compressive Strength"@en,
        "Résistance à la Compression"@fr .



me:tensileStrength a skos:Concept ;
    skos:broader me:mechanical ;
    skos:definition "The ability of a material to withstand tensile (pulling) forces without failure."@en ;
    skos:inScheme me:MyThesaurus ;
    skos:prefLabel "Zugfestigkeit"@de,
        "Tensile Strength"@en,
        "Résistance à la Traction"@fr .
        
me:youngsModulus a skos:Concept ;
    skos:broader me:mechanical ;
    skos:definition "A measure of the stiffness of a material, defined as the ratio of stress to strain in the linear elastic region."@en ;
    skos:inScheme me:MyThesaurus ;
    skos:prefLabel "E-Modul"@de,
        "Young's Modulus"@en,
        "Module d'élasticité"@fr .

me:hygrothermal a skos:Concept ;
    skos:broader me:Property ;
    skos:definition "Properties of materials related to their moisture and thermal behavior, such as thermal conductivity and moisture permeability."@en ;
    skos:inScheme me:MyThesaurus ;
    skos:prefLabel "Hygrothermisch"@de,
        "Hygrothermal"@en,
        "Hygrothermique"@fr .

me:thermalConductivity a skos:Concept ;
    skos:broader me:hygrothermal ;
    skos:definition "The ability of a material to conduct heat, defined as the amount of heat that passes through a unit area of the material per unit time for a given temperature difference."@en ;
    skos:inScheme me:MyThesaurus ;
    skos:prefLabel "Wärmeleitfähigkeit"@de,
        "Thermal Conductivity"@en,
        "Conductivité Thermique"@fr .

me:thermalCapacity a skos:Concept ;
    skos:broader me:hygrothermal ;
    skos:definition "The ability of a material to store thermal energy, defined as the amount of heat required to change the temperature of a unit mass of the material by one degree Celsius."@en ;
    skos:inScheme me:MyThesaurus ;
    skos:prefLabel "Wärmekapazität"@de,
        "Thermal Capacity"@en,
        "Capacité Thermique"@fr .

me:watervaporDiffusionResistance a skos:Concept ;
    skos:broader me:hygrothermal ;
    skos:definition "The resistance of a material to the diffusion of water vapor, defined as the ratio of the water vapor pressure difference across the material to the water vapor flux through the material."@en ;
    skos:inScheme me:MyThesaurus ;
    skos:prefLabel "Wasserdampfdiffusionswiderstand"@de,
        "Water vapor Diffusion Resistance"@en,
        "Résistance à la Diffusion de la Vapeur d'Eau"@fr .

me:moistureBufferingValue a skos:Concept ;
    skos:broader me:hygrothermal ;
    skos:definition "The ability of a material to buffer changes in moisture content, defined as the ratio of the change in moisture content to the change in relative humidity."@en ;
    skos:inScheme me:MyThesaurus ;
    skos:prefLabel "Feuchtepufferwert"@de,
        "Moisture Buffering Value"@en,
        "Valeur de Tampon d'Humidité"@fr .

me:porosity a skos:Concept ;
    skos:broader me:hygrothermal ;
    skos:definition "The ratio of the volume of voids in a material to the total volume of the material, expressed as a percentage."@en ;
    skos:inScheme me:MyThesaurus ;
    skos:prefLabel "Porosität"@de,
        "Porosity"@en,
        "Porosité"@fr .

me:effusivity a skos:Concept ;
    skos:broader me:hygrothermal ;
    skos:definition "A measure of a material's ability to exchange heat with its environment, defined as the square root of the product of thermal conductivity and volumetric heat capacity."@en ;
    skos:inScheme me:MyThesaurus ;
    skos:prefLabel "Effusivität"@de,
        "Effusivity"@en,
        "Effusivité"@fr .

me:waterContentAt80Percent a skos:Concept ;
    skos:broader me:hygrothermal ;
    skos:definition "The water content of a material at 80% relative humidity, expressed as a percentage of the dry mass of the material."@en ;
    skos:inScheme me:MyThesaurus ;
    skos:prefLabel "Wassergehalt bei 80% relativer Luftfeuchte"@de,
        "Water Content at 80% Relative Humidity"@en,
        "Teneur en Eau à 80% d'Humidité Relative"@fr .

me:freeSaturation a skos:Concept ;
    skos:broader me:hygrothermal ;
    skos:definition "The maximum amount of water that a material can absorb without any free water present, expressed as a percentage of the dry mass of the material."@en ;
    skos:inScheme me:MyThesaurus ;
    skos:prefLabel "Freie Sättigung"@de,
        "Free Saturation"@en,
        "Saturation Libre"@fr .

me:acoustic a skos:Concept ;
    skos:broader me:Property ;
    skos:definition "Properties of materials related to their acoustic behavior, such as sound absorption and sound insulation."@en ;
    skos:inScheme me:MyThesaurus ;
    skos:prefLabel "Akustisch"@de,
        "Acoustic"@en,
        "Acoustique"@fr .

me:absorptionCoefficientAt500Hz a skos:Concept ;
    skos:broader me:acoustic ;
    skos:definition "The sound absorption coefficient of a material at 500 Hz, defined as the ratio of the sound energy absorbed by the material to the total sound energy incident on the material."@en ;
    skos:inScheme me:MyThesaurus ;
    skos:prefLabel "Absorptionskoeffizient bei 500 Hz"@de,
        "Absorption Coefficient at 500 Hz"@en,
        "Coefficient d'Absorption à 500 Hz"@fr .
    
me:fireResistance a skos:Concept ;
    skos:broader me:Property ;
    skos:definition "The ability of a material to withstand fire or heat without significant degradation or failure."@en ;
    skos:inScheme me:MyThesaurus ;
    skos:prefLabel "Brandwiderstand"@de,
        "Fire Resistance"@en,
        "Résistance au Feu"@fr .

me:reactionToFireClassDINEN135011 a skos:Concept ;
    skos:broader me:fireResistance ;
    skos:definition "The classification of a material's reaction to fire according to the DIN EN 13501-1 standard, which assesses the fire performance of construction products."@en ;
    skos:inScheme me:MyThesaurus ;
    skos:prefLabel "Reaktion auf Feuer Klasse DIN EN 13501-1"@de,
        "Reaction to Fire Class DIN EN 13501-1"@en,
        "Classe de Réaction au Feu DIN EN 13501-1"@fr .

me:ApartmentBuilding a skos:Concept ;
    skos:broader me:Building ;
    skos:definition "Buildings sporting multiple storeys."@en ;
    skos:inScheme me:MyThesaurus ;
    skos:prefLabel "Mehrfamilienhaus"@de,
        "Multi-Storey Housing"@en,
        "Immeuble d'Habitation"@fr .

me:Architect a skos:Concept ;
    skos:broader me:Professional ;
    skos:definition "A professional responsible for designing buildings"@en ;
    skos:inScheme me:MyThesaurus ;
    skos:prefLabel "Architekt:in"@de,
        "Architect"@en,
        "Architecte"@fr .

me:AssociationProfessional a skos:Concept ;
    skos:broader me:Professional ;
    skos:definition "An organization promoting either a way of building or the professionals using it"@en ;
    skos:inScheme me:MyThesaurus ;
    skos:prefLabel "Verband/Verein"@de,
        "Association"@en,
        "Association"@fr .

me:Balcony a skos:Concept ;
    skos:broader me:Structure ;
    skos:definition "Structure outside exterior wall"@en ;
    skos:inScheme me:MyThesaurus ;
    skos:prefLabel "Balkon"@de,
        "Balcony"@en .

me:Bricks a skos:Concept ;
    skos:broader me:BuildingMaterial ;
    skos:definition "Blocks of various formats depending on density, preferences, available forms and purposes."@en ;
    skos:inScheme me:MyThesaurus ;
    skos:prefLabel "Baustein"@de,
        "Bricks"@en,
        "Briques"@fr .

me:BuildingPhysicsProfessional a skos:Concept ;
    skos:broader me:Professional ;
    skos:definition "A specialist focusing on the physical properties of buildings, including thermal, acoustic, and energy performance."@en ;
    skos:inScheme me:MyThesaurus ;
    skos:prefLabel "Bauphysiker:in"@de,
        "Building Physics"@en,
        "Physique du Bâtiment"@fr .

me:Bulk a skos:Concept ;
    skos:broader me:BuildingMaterial ;
    skos:definition "Loose building materials used to fill voids"@en ;
    skos:inScheme me:MyThesaurus ;
    skos:prefLabel "Schüttgut"@de,
        "Bulk"@en,
        "Vrac"@fr .

me:Ceiling a skos:Concept ;
    skos:broader me:Structure ;
    skos:definition "Separation between storeys"@en ;
    skos:inScheme me:MyThesaurus ;
    skos:prefLabel "Decke"@de,
        "Ceiling"@en .

me:CeilingFinishing a skos:Concept ;
    skos:broader me:Finishings ;
    skos:definition "Ceiling Finishing"@en ;
    skos:inScheme me:MyThesaurus ;
    skos:prefLabel "Deckenbekleidung"@de,
        "Ceiling Finishing"@en .

me:CivilEngineer a skos:Concept ;
    skos:broader me:Professional ;
    skos:definition "A professional specializing in the design, construction, and maintenance of infrastructure and buildings."@en ;
    skos:inScheme me:MyThesaurus ;
    skos:prefLabel "Bauingenieur:in"@de,
        "Civil engineer"@en,
        "Ingénieur civil"@fr .

me:Column a skos:Concept ;
    skos:broader me:Structure ;
    skos:definition "Load-bearing elements usually indoors"@en ;
    skos:inScheme me:MyThesaurus ;
    skos:prefLabel "Stütze"@de,
        "Column"@en .

me:ConstructionFirmProfessional a skos:Concept ;
    skos:broader me:Professional ;
    skos:definition "A company engaged in building construction projects and services."@en ;
    skos:inScheme me:MyThesaurus ;
    skos:prefLabel "Bauunternehmen"@de,
        "Construction Firm"@en,
        "Entreprise de Construction"@fr .

me:Craftsman a skos:Concept ;
    skos:broader me:Professional ;
    skos:definition "A skilled worker specializing in manual trades related to construction"@en ;
    skos:inScheme me:MyThesaurus ;
    skos:prefLabel "Handwerker:in"@de,
        "Craftsman"@en,
        "Artisan/ne"@fr .

me:Earth a skos:Concept ;
    skos:broader me:NaturalResource ;
    skos:definition "Naturally occuring resource in the sub-soil containing clay as binder for silts and sands in different proportions."@en ;
    skos:inScheme me:MyThesaurus ;
    skos:prefLabel "Lehm"@de,
        "Earth"@en,
        "Terre"@fr .

me:ExteriorThermalInsulation a skos:Concept ;
    skos:broader me:Envelope ;
    skos:definition "External Thermal Insulation"@en ;
    skos:inScheme me:MyThesaurus ;
    skos:prefLabel "Aussenwärmedämmung"@de,
        "Ext. Thermal Insulation"@en .

me:ExteriorWallAboveGround a skos:Concept ;
    skos:broader me:Structure ;
    skos:definition "Wall that separates the exterior from teh interior of the building above ground"@en ;
    skos:inScheme me:MyThesaurus ;
    skos:prefLabel "Aussenwand Über Terrain"@de,
        "Exterior Wall Above Ground"@en .

me:ExteriorWallFinishingAboveGround a skos:Concept ;
    skos:broader me:Envelope ;
    skos:definition "Facade finishing above ground"@en ;
    skos:inScheme me:MyThesaurus ;
    skos:prefLabel "Fassadenbekleidung"@de,
        "Ext. Wall Finishing Above Ground"@en .

me:ExteriorWallFinishingBasement a skos:Concept ;
    skos:broader me:Envelope ;
    skos:definition "External wall finishing under ground"@en ;
    skos:inScheme me:MyThesaurus ;
    skos:prefLabel "Äussere Beschichtung Unter Terrain"@de,
        "Ext. Wall Finishing Under Ground"@en .

me:ExteriorWallUnderGround a skos:Concept ;
    skos:broader me:Structure ;
    skos:definition "Wall that separates the exterior from teh interior of the building under ground"@en ;
    skos:inScheme me:MyThesaurus ;
    skos:prefLabel "Aussenwand Unter Terrain"@de,
        "Exterior Wall Under Ground"@en .

me:FloorCovering a skos:Concept ;
    skos:broader me:Finishings ;
    skos:definition "Floor Covering"@en ;
    skos:inScheme me:MyThesaurus ;
    skos:prefLabel "Bodenbelag"@de,
        "Floor Covering"@en .

me:FloorSlabGroundFloor a skos:Concept ;
    skos:broader me:Structure ;
    skos:definition "Slab that represents the floor at ground level"@en ;
    skos:inScheme me:MyThesaurus ;
    skos:prefLabel "Bodenplatte EG"@de,
        "Floor Slab Ground Floor"@en,
        "Dalle Rez-de-chaussée"@fr .

me:Foundation a skos:Concept ;
    skos:broader me:Structure ;
    skos:definition "Foundation of a structure, either underground or above, to transmit the forces applied by the structure to the ground, underground or bedrock"@en ;
    skos:inScheme me:MyThesaurus ;
    skos:prefLabel "Fundament"@de,
        "Foundation"@en .

me:Hemp a skos:Concept ;
    skos:broader me:NaturalResource ;
    skos:definition "Hemp"@en ;
    skos:inScheme me:MyThesaurus ;
    skos:prefLabel "Hanf"@de,
        "Hemp"@en,
        "Chanvre"@fr .

me:InteriorDoor a skos:Concept ;
    skos:broader me:Finishings ;
    skos:definition "Interior Door"@en ;
    skos:inScheme me:MyThesaurus ;
    skos:prefLabel "Innentür"@de,
        "Interior Door"@en .

me:InteriorWall a skos:Concept ;
    skos:broader me:Structure ;
    skos:definition "Structural wall inside the building"@en ;
    skos:inScheme me:MyThesaurus ;
    skos:prefLabel "Innenwand"@de,
        "Interior Wall"@en .

me:InteriorWallFinishing a skos:Concept ;
    skos:broader me:Finishings ;
    skos:definition "Interior Wall Finishing"@en ;
    skos:inScheme me:MyThesaurus ;
    skos:prefLabel "Wandbekleidung"@de,
        "Interior Wall Finishing"@en .

me:Massive a skos:Concept ;
    skos:broader me:BuildingMaterial ;
    skos:definition "Building Materials that can be processed to become massive, homogene building elements. They can be load-bearing or not and are mostly in need of formwork. "@en ;
    skos:inScheme me:MyThesaurus ;
    skos:prefLabel "Massivbau"@de,
        "Massive"@en,
        "Massif"@fr .

me:MaterialProducer a skos:Concept ;
    skos:broader me:Professional ;
    skos:definition "A company or individual involved in the production and supply of construction materials."@en ;
    skos:inScheme me:MyThesaurus ;
    skos:prefLabel "Materialhersteller:in"@de,
        "Material Producer"@en,
        "Producteur de Matériaux"@fr .

me:Mortar a skos:Concept ;
    skos:broader me:BuildingMaterial ;
    skos:definition "Mixes of a binder, fillers and sometimes additives to bond bricks or to plaster or render surfaces."@en ;
    skos:inScheme me:MyThesaurus ;
    skos:prefLabel "Mörtel, Putz"@de,
        "Mortar, Plaster"@en,
        "Mortier, Crépis"@fr .

me:NewBuilding a skos:Concept ;
    skos:broader me:Building,
        me:BuildingStatus ;
    skos:definition "Buildings that were newly constructed."@en ;
    skos:inScheme me:MyThesaurus ;
    skos:prefLabel "Neu"@de,
        "New"@en,
        "Nouveau"@fr .

me:OfficeBuilding a skos:Concept ;
    skos:broader me:Building ;
    skos:definition "Buildings primarily used for commercial office purposes."@en ;
    skos:inScheme me:MyThesaurus ;
    skos:prefLabel "Bürogebäude"@de,
        "Office Building"@en,
        "Immeuble de Bureaux"@fr .

me:OtherFibers a skos:Concept ;
    skos:broader me:NaturalResource ;
    skos:definition "Fibrous plants other than cereals or hemp"@en ;
    skos:inScheme me:MyThesaurus ;
    skos:prefLabel "Andere Fasern"@de,
        "Other Fibres"@en,
        "Autres fibres"@fr .

me:Panels a skos:Concept ;
    skos:broader me:BuildingMaterial ;
    skos:definition "Prefabricated flat building materials, designed for different purposes as panelling and/or insulation"@en ;
    skos:inScheme me:MyThesaurus ;
    skos:prefLabel "Platten"@de,
        "Panels, Boards"@en,
        "Plaques"@fr .

me:PartitionWall a skos:Concept ;
    skos:broader me:Finishings ;
    skos:definition "Partition Wall, non load-bearing"@en ;
    skos:inScheme me:MyThesaurus ;
    skos:prefLabel "Trennwand"@de,
        "Partition Wall"@en .

me:PublicBuilding a skos:Concept ;
    skos:broader me:Building ;
    skos:definition "Buildings intended for use by the public, such as schools, libraries, or government offices."@en ;
    skos:inScheme me:MyThesaurus ;
    skos:prefLabel "Öffentliches Gebäude"@de,
        "Public Building"@en,
        "Bâtiment Public"@fr .

me:RenovationBuilding a skos:Concept ;
    skos:broader me:Building,
        me:BuildingStatus ;
    skos:definition "Buildings that underwent repair or adaptation to new needs."@en ;
    skos:inScheme me:MyThesaurus ;
    skos:prefLabel "Umbau"@de,
        "Renovation"@en,
        "Rénovation"@fr .

me:Researcher a skos:Concept ;
    skos:broader me:Professional ;
    skos:definition "A academic or industrial researcher with expertise in regenerative materials"@en ;
    skos:inScheme me:MyThesaurus ;
    skos:prefLabel "Forscher:in"@de,
        "Researcher"@en,
        "Chercheur/se"@fr .

me:Reseller a skos:Concept ;
    skos:broader me:Professional ;
    skos:definition "Company or individual reselling building materials "@en ;
    skos:inScheme me:MyThesaurus ;
    skos:prefLabel "Händler:in"@de,
        "Reseller"@en,
        "Revendeur/se"@fr .

me:Rock a skos:Concept ;
    skos:broader me:NaturalResource ;
    skos:definition "Natural rocks that can be found the bedrock"@en ;
    skos:inScheme me:MyThesaurus ;
    skos:prefLabel "Gestein"@de,
        "Rock"@en,
        "Roche"@fr .

me:Roof a skos:Concept ;
    skos:broader me:Structure ;
    skos:definition "Roof construction load-bearing"@en ;
    skos:inScheme me:MyThesaurus ;
    skos:prefLabel "Dach"@de,
        "Roof"@en .

me:RoofCovering a skos:Concept ;
    skos:broader me:Envelope ;
    skos:definition "Roof Covering"@en ;
    skos:inScheme me:MyThesaurus ;
    skos:prefLabel "Bedachung"@de,
        "Roof Covering"@en .

me:SimpleStructure a skos:Concept ;
    skos:broader me:Building ;
    skos:definition "Basic or minimal buildings or structures, typically with limited complexity or use."@en ;
    skos:inScheme me:MyThesaurus ;
    skos:prefLabel "Einfache Struktur"@de,
        "Simple Structure"@en,
        "Structure Simple"@fr .

me:SingleFamilyHouse a skos:Concept ;
    skos:broader me:Building ;
    skos:definition "Buildings intended for a smaller amount of inhabitants"@en ;
    skos:inScheme me:MyThesaurus ;
    skos:prefLabel "Einfamilienhaus"@de,
        "Single Family House"@en,
        "Maison Individuelle"@fr .

me:Stair a skos:Concept ;
    skos:broader me:Structure ;
    skos:definition "Stair"@en ;
    skos:inScheme me:MyThesaurus ;
    skos:prefLabel "Treppe"@de,
        "Stair"@en .

me:Straw a skos:Concept ;
    skos:broader me:NaturalResource ;
    skos:definition "Dried stalks of cereals"@en ;
    skos:inScheme me:MyThesaurus ;
    skos:prefLabel "Stroh"@de,
        "Straw"@en,
        "Paille"@fr .

me:SunWeatherProtection a skos:Concept ;
    skos:broader me:Envelope ;
    skos:definition "Sun & Weather Protection"@en ;
    skos:inScheme me:MyThesaurus ;
    skos:prefLabel "Sonnen- & Wetterschutz"@de,
        "Sun & Weather Protection"@en .

me:TechnicalEquipement a skos:Concept ;
    skos:broader me:Other ;
    skos:definition "Technical Equipement as Heating, Ventilation, Water or electricity supply"@en ;
    skos:inScheme me:MyThesaurus ;
    skos:prefLabel "Technik"@de,
        "Technical Equipement"@en .

me:Timber a skos:Concept ;
    skos:broader me:BuildingMaterial ;
    skos:definition "Timber"@en ;
    skos:inScheme me:MyThesaurus ;
    skos:prefLabel "Timber"@en .

me:WindowDoor a skos:Concept ;
    skos:broader me:Envelope ;
    skos:definition "Windows and doors in envelope"@en ;
    skos:inScheme me:MyThesaurus ;
    skos:prefLabel "Fenster & Türen"@de,
        "Windows & Doors"@en .

me:Wood a skos:Concept ;
    skos:broader me:NaturalResource ;
    skos:definition "Wood"@en ;
    skos:inScheme me:MyThesaurus ;
    skos:prefLabel "Holz"@de,
        "Wood"@en,
        "Bois"@fr .

me:Other a skos:Concept ;
    skos:broader me:TechnicalConstruction ;
    skos:definition "Other concepts not fitting into the main categories of the AREMA Ontology."@en ;
    skos:inScheme me:MyThesaurus ;
    skos:prefLabel "Andere"@de,
        "Other"@en,
        "Autre"@fr .

me:BuildingStatus a skos:Concept ;
    skos:broader me:Building ;
    skos:definition "Classification of buildings based on the type of intervention, such as new construction or renovation."@en ;
    skos:inScheme me:MyThesaurus ;
    skos:prefLabel "Art der Massnahme"@de,
        "Intervention Type"@en,
        "Type d'Intervention"@fr .

me:Finishings a skos:Concept ;
    skos:broader me:TechnicalConstruction ;
    skos:definition "Finishing elements of a building, such as wall coverings, floor coverings, and ceiling finishes."@en ;
    skos:inScheme me:MyThesaurus ;
    skos:prefLabel "Oberflächen"@de,
        "Finishings"@en,
        "Finitions"@fr .

me:TechnicalConstruction a skos:Concept ;
    skos:broader me:Object ;
    skos:definition "Techniques used to assemble building materials to become building elements."@en ;
    skos:inScheme me:MyThesaurus ;
    skos:prefLabel "Bauweise"@de,
        "Construction Techniques"@en,
        "Systèmes Constructifs"@fr .

me:Envelope a skos:Concept ;
    skos:broader me:TechnicalConstruction ;
    skos:definition """The outer shell of a building, including walls, roofs, and windows, that separates the interior from the exterior environment."""@en ;
    skos:inScheme me:MyThesaurus ;
    skos:prefLabel "Hülle"@de,
        "Envelope"@en,
        "Enveloppe"@fr .

me:BuildingMaterial a skos:Concept ;
    skos:broader me:Object ;
    skos:definition "Materials made out of resources by transformation and processing for the purpose of building."@en ;
    skos:inScheme me:MyThesaurus ;
    skos:prefLabel "Baustoffe"@de,
        "Building Materials"@en,
        "Matériaux de Construction"@fr .

me:NaturalResource a skos:Concept ;
    skos:broader me:Object ;
    skos:definition "Resources that can potentially be used for construction; both occuring naturally (like bio- or geo-sourced) or being salvaged from demoltions."@en ;
    skos:inScheme me:MyThesaurus ;
    skos:prefLabel "Ressourcen"@de,
        "Resources"@en,
        "Ressources"@fr .

me:Building a skos:Concept ;
    skos:broader me:Object ;
    skos:definition "Exemplary buildings or structures made with a earnest commitment to using regenerative materials."@en ;
    skos:inScheme me:MyThesaurus ;
    skos:prefLabel "Gebäude"@de,
        "Buildings"@en,
        "Bâtiments"@fr .

me:Professional a skos:Concept ;
    skos:broader me:Object ;
    skos:definition "Persons or organizations providing services or materials around regenerative materials."@en ;
    skos:inScheme me:MyThesaurus ;
    skos:prefLabel "Fachleute"@de,
        "Professionals"@en,
        "Professionnels"@fr .

me:Structure a skos:Concept ;
    skos:broader me:TechnicalConstruction ;
    skos:definition "A structure"@en ;
    skos:inScheme me:MyThesaurus ;
    skos:prefLabel "Struktur"@de,
        "Structure"@en,
        "Structure"@fr .

me:Property a skos:Concept ;
    skos:definition "Properties of building materials."@en ;
    skos:inScheme me:MyThesaurus ;
    skos:prefLabel "Eigenschaften"@de,
        "Properties"@en,
        "Propriétés"@fr .

me:Object a skos:Concept ;
    skos:definition "A physical entity that can be described or measured, such as a building material or a structure."@en ;
    skos:inScheme me:MyThesaurus ;
    skos:prefLabel "Objekt"@de,
        "Object"@en,
        "Objet"@fr .
        
me:MyThesaurus a skos:ConceptScheme ;
    dct:description "AREMA Ontology for building materials, buildings, natural resources, professionals, and technical constructions."@en ;
    dct:license <https://creativecommons.org/licenses/by/4.0/> ;
    vann:preferredNamespacePrefix "me" ;
    vann:preferredNamespaceUri "https://w3id.org/arema/ontology/" ;
    skos:hasTopConcept me:Object, me:Property ;
    skos:prefLabel "AREMA Ontologie"@de,
        "AREMA Ontology"@en,
        "Ontologie AREMA"@fr,
        "Ontologia AREMA"@it .


