@prefix rdfs: <http://www.w3.org/2000/01/rdf-schema#> .
@prefix me: <http://example.org/taxonomy/> .
@prefix brick: <https://w3id.org/brick#> .
@prefix ifc: <https://standards.buildingsmart.org/IFC/DEV/IFC4/ADD2_TC1/OWL#> .
@prefix owl: <http://www.w3.org/2002/07/owl#> .
@prefix skos: <http://www.w3.org/2004/02/skos/core#> .
@prefix xsd: <http://www.w3.org/2001/XMLSchema#> .
@prefix dct: <http://purl.org/dc/terms/>.
@prefix vann: <http://purl.org/vocab/vann/> .

@base <https://w3id.org/arema/ontology/>.


me:MyThesaurus a skos:ConceptScheme ;
    skos:prefLabel "AREMA Ontology"@en ;
    dct:description "AREMA Ontology for building materials, buildings, natural resources, professionals, and technical constructions."@en ;
    vann:preferredNamespaceUri "https://w3id.org/arema/ontology/" ;
    vann:preferredNamespacePrefix "me" ;
    skos:hasTopConcept me:BuildingMaterial, me:Building, me:NaturalResource, me:Professional, me:TechnicalConstruction ;
    skos:prefLabel "AREMA Ontology"@en , "AREMA Ontologie"@de , "Ontologie AREMA"@fr , "Ontologia AREMA"@it ;
    dct:license <https://creativecommons.org/licenses/by/4.0/> .

# Top-level classes (formerly Concept Schemes)
me:BuildingMaterial a skos:Concept ;
skos:inScheme me:MyThesaurus ;
skos:prefLabel "Building Materials"@en , "Baustoffe"@de , "Matériaux de construction"@fr , "Materiali da costruzione"@it .
me:Building a skos:Concept ;
skos:inScheme me:MyThesaurus ;
skos:prefLabel "Buildings"@en , "Gebäude"@de , "Bâtiments"@fr , "Edifici"@it .
me:NaturalResource a skos:Concept ;
skos:inScheme me:MyThesaurus ;
skos:prefLabel "Natural Resources"@en , "Natürliche Ressourcen"@de , "Ressources naturelles"@fr , "Risorse naturali"@it .
me:Professional a skos:Concept ;
skos:inScheme me:MyThesaurus ;
skos:prefLabel "Professionals"@en , "Fachleute"@de , "Professionnels"@fr , "Professionisti"@it .
me:TechnicalConstruction a skos:Concept ;
skos:inScheme me:MyThesaurus ;
skos:prefLabel "Technical Constructions"@en , "Technische Konstruktionen"@de , "Constructions techniques"@fr , "Costruzioni tecniche"@it ;
    skos:definition "Aspects of construction related to the physical realization of buildings, encompassing structural, thermal, acoustic, and service-related elements."@en .

# Building Materials Taxonomy
me:Massive skos:broader me:BuildingMaterial ;
    a skos:Concept ;
skos:inScheme me:MyThesaurus ;
skos:prefLabel "Massive"@en , "Massivlehmbau"@de , "Massif"@fr , "Massiccio"@it .

me:Bricks skos:broader me:BuildingMaterial ;
    a skos:Concept ;
skos:inScheme me:MyThesaurus ;
skos:prefLabel "Bricks"@en , "Baustein"@de , "Briques"@fr , "Mattoni"@it .

me:Panels skos:broader me:BuildingMaterial ;
    a skos:Concept ;
skos:inScheme me:MyThesaurus ;
skos:prefLabel "Panels, Boards"@en , "Platten"@de , "Plaques"@fr , "Pannelli"@it .

me:Bulk skos:broader me:BuildingMaterial ;
    a skos:Concept ;
skos:inScheme me:MyThesaurus ;
skos:prefLabel "Bulk"@en , "Schüttgut"@de , "Vrac"@fr , "Massa"@it .

me:Mortar skos:broader me:BuildingMaterial ;
    a skos:Concept ;
skos:inScheme me:MyThesaurus ;
skos:prefLabel "Mortar, Plaster"@en , "Mörtel, Putz"@de , "Mortier, Crépis"@fr , "Malta, Intonaco"@it .

# Buildings Taxonomy
me:BuildingStatus skos:broader me:Building ;
    a skos:Concept ;
skos:inScheme me:MyThesaurus ;
skos:prefLabel "Building Status"@en , "Gebäudestatus"@de , "Statut du bâtiment"@fr , "Stato dell'edificio"@it .

me:NewBuilding skos:broader me:BuildingStatus ;
    a skos:Concept ;
skos:inScheme me:MyThesaurus ;
skos:prefLabel "New"@en , "Neu"@de , "Nouveau"@fr , "Nuovo"@it .

me:RenovationBuilding skos:broader me:BuildingStatus ;
    a skos:Concept ;
skos:inScheme me:MyThesaurus ;
skos:prefLabel "Renovation"@en , "Renovierung"@de , "Rénovation"@fr , "Ristrutturazione"@it .

me:ApartmentBuilding skos:broader me:Building ;
    a skos:Concept ;
skos:inScheme me:MyThesaurus ;
skos:prefLabel "Apartment Building"@en , "Mehrfamilienhaus"@de , "Immeuble d'habitation"@fr , "Edificio residenziale"@it .

me:SingleFamilyHouse skos:broader me:Building ;
    a skos:Concept ;
skos:inScheme me:MyThesaurus ;
skos:prefLabel "Single Family House"@en , "Einfamilienhaus"@de , "Maison individuelle"@fr , "Casa unifamiliare"@it .

me:OfficeBuilding skos:broader me:Building ;
    a skos:Concept ;
skos:inScheme me:MyThesaurus ;
skos:prefLabel "Office Building"@en , "Bürogebäude"@de , "Immeuble de bureaux"@fr , "Edificio per uffici"@it .

me:PublicBuilding skos:broader me:Building ;
    a skos:Concept ;
skos:inScheme me:MyThesaurus ;
skos:prefLabel "Public Building"@en , "Öffentliches Gebäude"@de , "Bâtiment public"@fr , "Edificio pubblico"@it .

me:SimpleStructure skos:broader me:Building ;
    a skos:Concept ;
skos:inScheme me:MyThesaurus ;
skos:prefLabel "Simple Structure"@en , "Einfache Struktur"@de , "Structure simple"@fr , "Struttura semplice"@it .

# Natural Resources Taxonomy
me:Earth skos:broader me:NaturalResource ;
    a skos:Concept ;
skos:inScheme me:MyThesaurus ;
skos:prefLabel "Earth"@en , "Erde"@de , "Terre"@fr , "Terra"@it .

me:Rock skos:broader me:NaturalResource ;
    a skos:Concept ;
skos:inScheme me:MyThesaurus ;
skos:prefLabel "Rock"@en , "Gestein"@de , "Roche"@fr , "Rocce"@it .

me:Straw skos:broader me:NaturalResource ;
    a skos:Concept ;
skos:inScheme me:MyThesaurus ;
skos:prefLabel "Straw"@en , "Stroh"@de , "Paille"@fr , "Paglia"@it .

me:Hemp skos:broader me:NaturalResource ;
    a skos:Concept ;
skos:inScheme me:MyThesaurus ;
skos:prefLabel "Hemp"@en , "Hanf"@de , "Chanvre"@fr , "Canapa"@it .

me:Wood skos:broader me:NaturalResource ;
    a skos:Concept ;
skos:inScheme me:MyThesaurus ;
skos:prefLabel "Wood"@en , "Holz"@de , "Bois"@fr , "Legno"@it .

me:OtherFibers skos:broader me:NaturalResource ;
    a skos:Concept ;
skos:inScheme me:MyThesaurus ;
skos:prefLabel "Other Fibers"@en , "Andere Fasern"@de , "Autres fibres"@fr , "Altre fibre"@it .

# Professionals Taxonomy
me:Architect skos:broader me:Professional ;
    a skos:Concept ;
skos:inScheme me:MyThesaurus ;
skos:prefLabel "Architect"@en , "Architekt"@de , "Architecte"@fr , "Architetto"@it .

me:CivilEngineer skos:broader me:Professional ;
    a skos:Concept ;
skos:inScheme me:MyThesaurus ;
skos:prefLabel "Civil engineer"@en , "Bauingenieur"@de , "Ingénieur civil"@fr , "Ingegnere civile"@it .

me:Craftsman skos:broader me:Professional ;
    a skos:Concept ;
skos:inScheme me:MyThesaurus ;
skos:prefLabel "Craftsman"@en , "Handwerker"@de , "Artisan"@fr , "Artigiano"@it .

me:MaterialProducer skos:broader me:Professional ;
    a skos:Concept ;
skos:inScheme me:MyThesaurus ;
skos:prefLabel "Material Producer"@en , "Materialhersteller"@de , "Producteur de matériaux"@fr , "Produttore di materiali"@it .

me:BuildingPhysicsProfessional skos:broader me:Professional ;
    a skos:Concept ;
skos:inScheme me:MyThesaurus ;
skos:prefLabel "Building Physics"@en , "Bauphysik"@de , "Physique du bâtiment"@fr , "Fisica dell'edificio"@it .

me:AssociationProfessional skos:broader me:Professional ;
    a skos:Concept ;
skos:inScheme me:MyThesaurus ;
skos:prefLabel "Association"@en , "Verband"@de , "Association"@fr , "Associazione"@it .

me:ConstructionFirmProfessional skos:broader me:Professional ;
    a skos:Concept ;
skos:inScheme me:MyThesaurus ;
skos:prefLabel "Construction Firm"@en , "Bauunternehmen"@de , "Entreprise de construction"@fr , "Impresa di costruzioni"@it .

me:ResearcherProfessional skos:broader me:Professional ;
    a skos:Concept ;
skos:inScheme me:MyThesaurus ;
skos:prefLabel "Researcher"@en , "Forscher"@de , "Chercheur"@fr , "Ricercatore"@it .

me:ResellerProfessional skos:broader me:Professional ;
    a skos:Concept ;
skos:inScheme me:MyThesaurus ;
skos:prefLabel "Reseller"@en , "Wiederverkäufer"@de , "Revendeur"@fr , "Rivenditore"@it .

me:ProfessionalOther skos:broader me:Professional ;
    a skos:Concept ;
skos:inScheme me:MyThesaurus ;
skos:prefLabel "Other"@en , "Andere"@de , "Autre"@fr , "Altro"@it .


me:ConstructionWorker
    skos:broader me:Professional ;
    a skos:Concept ;
skos:inScheme me:MyThesaurus ;
skos:prefLabel "Construction Worker"@en , "Bauarbeiter"@de , "Ouvrier du bâtiment"@fr , "Operaio edile"@it ;
.

me:BuildingInspector
    skos:broader me:Professional ;
    a skos:Concept ;
skos:inScheme me:MyThesaurus ;
skos:prefLabel "Building Inspector"@en , "Bauinspektor"@de , "Inspecteur du bâtiment"@fr , "Ispettore edilizio"@it ;
.

# Technical Constructions Taxonomy
me:FireProtection skos:broader me:TechnicalConstruction ;
    a skos:Concept ;
skos:inScheme me:MyThesaurus ;
skos:prefLabel "Fire Protection"@en , "Brandschutz"@de , "Protection incendie"@fr , "Protezione antincendio"@it ;
    skos:definition "Measures and design elements intended to prevent, contain, and mitigate the effects of fire within a building."@en .

me:ThermalInsulation skos:broader me:TechnicalConstruction ;
    a skos:Concept ;
skos:inScheme me:MyThesaurus ;
skos:prefLabel "Thermal Insulation"@en , "Wärmeschutz"@de , "Isolation thermique"@fr , "Isolamento termico"@it ;
    skos:definition "Techniques and materials used to reduce the transfer of heat between the inside and outside of a building."@en .

me:MoistureProtection skos:broader me:TechnicalConstruction ;
    a skos:Concept ;
skos:inScheme me:MyThesaurus ;
skos:prefLabel "Moisture Protection"@en , "Feuchteschutz"@de , "Protection contre l'humidité"@fr , "Protezione dall'umidità"@it ;
    skos:definition "Strategies and components used to prevent moisture infiltration and control humidity in building structures."@en .

me:SoundInsulation skos:broader me:TechnicalConstruction ;
    a skos:Concept ;
skos:inScheme me:MyThesaurus ;
skos:prefLabel "Sound Insulation"@en , "Schallschutz"@de , "Isolation acoustique"@fr , "Isolamento acustico"@it ;
    skos:definition "Methods and materials designed to reduce the transmission of sound between and within building spaces."@en .

me:LoadBearingStructure skos:broader me:TechnicalConstruction ;
    a skos:Concept ;
skos:inScheme me:MyThesaurus ;
skos:prefLabel "Load-bearing Structure"@en , "Tragkonstruktion"@de , "Structure porteuse"@fr , "Struttura portante"@it ;
    skos:definition "The system of structural elements that support and transfer the weight and forces of a building to the ground."@en .

me:LightweightConstruction skos:broader me:TechnicalConstruction ;
    a skos:Concept ;
skos:inScheme me:MyThesaurus ;
skos:prefLabel "Lightweight Construction"@en , "Leichtbau"@de , "Construction légère"@fr , "Costruzione leggera"@it ;
    skos:definition "Construction techniques emphasizing minimal material usage and weight while maintaining structural integrity."@en .

me:BuildingServices skos:broader me:TechnicalConstruction ;
    a skos:Concept ;
skos:inScheme me:MyThesaurus ;
skos:prefLabel "Building Services"@en , "Technische Gebäudeausrüstung"@de , "Services du bâtiment"@fr , "Impianti tecnici dell'edificio"@it ;
    skos:definition "Technical systems installed in buildings, such as heating, ventilation, plumbing, and electrical infrastructure."@en .

me:BuildingEnvelope skos:broader me:TechnicalConstruction ;
    a skos:Concept ;
skos:inScheme me:MyThesaurus ;
skos:prefLabel "Building Envelope"@en , "Gebäudehülle"@de , "Enveloppe du bâtiment"@fr , "Involucro edilizio"@it ;
    skos:definition "The physical separator between the interior and exterior of a building, including walls, roofs, and windows."@en .

me:Prefabrication skos:broader me:TechnicalConstruction ;
    a skos:Concept ;
skos:inScheme me:MyThesaurus ;
skos:prefLabel "Prefabrication"@en , "Vorproduktion"@de , "Préfabrication"@fr , "Prefabbricazione"@it ;
    skos:definition "The process of manufacturing building components off-site for later assembly on-site."@en .

me:RenovationTechnicalConstruction skos:broader me:TechnicalConstruction ;
    a skos:Concept ;
skos:inScheme me:MyThesaurus ;
skos:prefLabel "Renovation"@en , "Sanierung"@de , "Rénovation"@fr , "Ristrutturazione"@it ;
    skos:definition "The process of improving, modernizing, or restoring an existing building."@en .

me:Deconstruction skos:broader me:TechnicalConstruction ;
    a skos:Concept ;
skos:inScheme me:MyThesaurus ;
skos:prefLabel "Deconstruction"@en , "Rückbau"@de , "Déconstruction"@fr , "Decostruzione"@it ;
    skos:definition "The systematic dismantling of a building with the goal of preserving materials for reuse or recycling."@en .

me:TechnicalConstructionOther skos:broader me:TechnicalConstruction ;
    a skos:Concept ;
skos:inScheme me:MyThesaurus ;
skos:prefLabel "Other"@en , "Andere"@de , "Autre"@fr , "Altro"@it ;
    skos:definition "Technical construction topics not covered by the predefined categories."@en .

# Building Materials
# me:BuildingMaterial
#     #skos:related ifc:IfcMaterial
#     .

me:Concrete a skos:Concept ;
    skos:inScheme me:MyThesaurus ;
    skos:prefLabel "Concrete"@en , "Beton"@de , "Béton"@fr , "Calcestruzzo"@it ;
    skos:broader me:BuildingMaterial ;
    .

me:moreSpecificTypeOfConcrete a skos:Concept ;
    skos:inScheme me:MyThesaurus ;
    skos:prefLabel "More Specific Type of Concrete"@en , "Spezifischer Beton"@de , "Type de béton plus spécifique"@fr , "Tipo di calcestruzzo più specifico"@it ;
    skos:broader me:Concrete ;
    .

me:Glass a skos:Concept ;
    skos:inScheme me:MyThesaurus ;
    skos:prefLabel "Glass"@en , "Glas"@de , "Verre"@fr , "Vetro"@it ;
    skos:broader me:BuildingMaterial ;
    .

me:Steel a skos:Concept ;
    skos:inScheme me:MyThesaurus ;
    skos:prefLabel "Steel"@en , "Stahl"@de , "Acier"@fr , "Acciaio"@it ;
    skos:broader me:BuildingMaterial ;
    .

me:Wood a skos:Concept ;
    skos:inScheme me:MyThesaurus ;
    skos:prefLabel "Wood"@en , "Holz"@de , "Bois"@fr , "Legno"@it ;
    skos:broader me:BuildingMaterial ;
    .
    
# Building Types
me:Building
    owl:equivalentClass brick:Building ;
    owl:equivalentClass ifc:IfcBuilding .

me:ApartmentBuilding
    skos:broader me:Building ;
    #skos:related ifc:IfcBuilding .
    .

me:OfficeBuilding
    skos:broader me:Building ;
    #skos:related ifc:IfcBuilding .
.
me:SingleFamilyHouse
    skos:broader me:Building ;
    #skos:related ifc:IfcBuilding .
.
# Technical Constructions
# me:TechnicalConstruction
#     #skos:related ifc:IfcElement .
# .
me:LoadBearingStructure
    skos:broader me:TechnicalConstruction ;
    #skos:related ifc:IfcStructuralElement .
.
me:ThermalInsulation
    skos:broader me:TechnicalConstruction ;
    #skos:related ifc:IfcMaterialLayer .
.
me:SoundInsulation
    skos:broader me:TechnicalConstruction ;
    #skos:related ifc:IfcMaterialLayer .
.
me:FireProtection
    skos:broader me:TechnicalConstruction ;
    #skos:related ifc:IfcFireSuppressionTerminal .
.
me:MoistureProtection
    skos:broader me:TechnicalConstruction ;
    #skos:related ifc:IfcCovering .
.
# Professionals
# me:Professional
#     #skos:related ifc:IfcActor .
# .


me:BuildingMaterial skos:definition "Materials used for construction purposes, including natural and manufactured substances."@en .

me:Building skos:definition "Physical structures intended for human use or occupancy, such as houses, offices, and public buildings."@en .

me:NaturalResource skos:definition "Naturally occurring substances or materials that can be used for construction, manufacturing, or energy production."@en .

me:Professional skos:definition "Persons or organizations providing expertise or services within the construction or building sectors."@en .

me:TechnicalConstruction skos:definition "Aspects of construction related to the physical realization of buildings, encompassing structural, thermal, acoustic, and service-related elements."@en .

me:Massive skos:definition "Building materials characterized by their mass and solidity, such as concrete or rammed earth."@en .

me:Bricks skos:definition "Modular building materials typically made of fired clay or similar substances, used in masonry construction."@en .

me:Panels skos:definition "Prefabricated flat building components, often used for walls, floors, and ceilings."@en .

me:Bulk skos:definition "Loose construction materials used in large quantities, such as gravel or sand."@en .

me:Mortar skos:definition "A mixture used in masonry to bond bricks, stones, or concrete blocks together."@en .

me:BuildingStatus skos:definition "Classification of buildings based on the type of intervention, such as new construction or renovation."@en .

me:NewBuilding skos:definition "Buildings that are newly constructed and not previously used or occupied."@en .

me:RenovationBuilding skos:definition "Buildings undergoing repair, improvement, or modernization."@en .

me:ApartmentBuilding skos:definition "Buildings containing multiple separate residential units."@en .

me:SingleFamilyHouse skos:definition "Residential buildings designed for occupancy by a single family."@en .

me:OfficeBuilding skos:definition "Buildings primarily used for commercial office purposes."@en .

me:PublicBuilding skos:definition "Buildings intended for use by the public, such as schools, libraries, or government offices."@en .

me:SimpleStructure skos:definition "Basic or minimal buildings or structures, typically with limited complexity or use."@en .

me:Earth skos:definition "Soil or clay materials used in construction, often in traditional building techniques."@en .

me:Rock skos:definition "Natural stone materials used in construction for strength and durability."@en .

me:Straw skos:definition "Dried stalks of grain plants used as a natural building material, often in combination with earth."@en .

me:Hemp skos:definition "Fibrous plant material used for insulation, blocks, and other eco-friendly construction purposes."@en .

me:Wood skos:definition "Timber or lumber derived from trees, commonly used in building structures and finishes."@en .

me:OtherFibers skos:definition "Various plant-based or synthetic fibers used as components in construction materials."@en .

me:Architect skos:definition "A professional responsible for designing buildings and overseeing their construction."@en .

me:CivilEngineer skos:definition "A professional specializing in the design, construction, and maintenance of infrastructure and buildings."@en .

me:Craftsman skos:definition "A skilled worker specializing in manual trades related to construction, such as carpentry or masonry."@en .

me:MaterialProducer skos:definition "A company or individual involved in the production and supply of construction materials."@en .

me:BuildingPhysicsProfessional skos:definition "A specialist focusing on the physical properties of buildings, including thermal, acoustic, and energy performance."@en .

me:AssociationProfessional skos:definition "An organization representing the interests of professionals within the construction sector."@en .

me:ConstructionFirmProfessional skos:definition "A company engaged in building construction projects and services."@en .
